\section{Calculus}
\subsection{Limit}
\begin{fact}{L'HÃ´pital's rule}{lhopital}
  Suppose that ($\lim\limits_{x\rightarrow a}f(x)=0$, $\lim\limits_{x\rightarrow a}g(x)=0$) or ($\lim\limits_{x\rightarrow a}f(x)=\infty$, $\lim\limits_{x\rightarrow a}g(x)=\infty$) and that $\lim\limits_{x\rightarrow a}\frac{f'(x)}{g'(x)}$ exists.
  Then
  \[
   \lim\limits_{x\rightarrow a}\frac{f(x)}{g(x)} = \lim\limits_{x\rightarrow a}\frac{f'(x)}{g'(x)}
  \]
\end{fact}

\subsection{Integration Methods}
\begin{fact}{Integration by parts}{intByPart}
  If $f'$ and $g'$ are continuous on $[a,b]$ then
\begin{align*}
   \int_{a}^{b} f'(t)g(t) dt & = \int_{a}^{b} f'(t)g'(t)\,dt - \int_{a}^{b} f(t)g'(t)\,dt\\
                             & = f(b)g(b)-f(a)g(a) - \int_{a}^{b} f(t)g'(t)\,dt.
\end{align*}

For indefinite integrals,
\[
  \int f'(t)g(t) dt = f(t)g(t) - \int f(t)g'(t)\,dt.
\]
\end{fact}

\begin{exec}
  Calculate $\int e^x \sin{x} dx$.
  \tcblower
  Factor $e^x\sin{x} = f'(x)g(x)$ into $f'(x) =e^x$ and $g(x)=\sin{x}$,
  where $f(x)=e^x$ and $g'(x)=\cos{x}$.
  \begin{align*}
    \int e^x \sin{x} dx = e^x \sin{x} - \int e^x \cos{x}\,dx
  \end{align*}
  Apply \nameref*{fact:intByPart} again for $\int e^x \cos{x}\,dx$,
  where $f'(x)=e^x$ \g $f(x)=e^x$ and $g(x)=\cos{x}$ \g $g'(x)=-\sin{x}$.
  \begin{align*}
    \int e^x \sin{x} dx &= e^x \sin{x} - (e^x\cos{x}-\int e^x (-\sin{x},dx))\\
    2\int e^x \sin{x} dx &= e^x \sin{x} - e^x\cos{x} \\
    \int e^x \sin{x} dx &= \frac{e^x}{2} \left(\sin{x} - \cos{x}\right)
  \end{align*}
\end{exec}

\begin{exec}
  Prove that $\int_{0}^{\infty}\frac{x^n}{e^{x}}\,dx = n!$, where $n$ is positive integer.
  \tcblower
  \begin{proof}
  Let $I_n = \int_{0}^{\infty}\frac{x^n}{e^{x}}\,dx$.

  Let $f'(x)=e^{-x}$\g$f(x)=-e^{-x}$ and $g(x)=x^n$\g$g'(x)=nx^{n-1}$, therefore
  \begin{align*}
    I_n = \int_{0}^{\infty}\frac{x^n}{e^{x}}\,dx
      &= \left[-e^{-x}nx^{n-1}\right]^{\infty}_{0} - \int_{0}^{\infty}-e^{-x}nx^{n-1} \\
      &= \left[\lim_{x\rightarrow\infty}e^{-x}(-nx^{n-1})\right] + n\int_{0}^{\infty}e^{-x}x^{n-1} \\
      &= nI_{n-1}
  \end{align*}
  Note that $\lim_{x\rightarrow\infty}e^{-x}p(x)=0$ for any polynomial function $p(x)$. Easily provable using \nameref{fact:lhopital}.

  Also $I_{0}=\int^{\infty}_{0}\frac{1}{e^x}=\left[-e^{-x}\right]^{\infty}_{0}=1$.

  Therefore $\int_{0}^{\infty}\frac{x^n}{e^{x}}\,dx=n!$ using proof by induction.
  \end{proof}
\end{exec}